Weidenbach_Book/IsaSAT/IsaSAT_Stats.thy
@@ -45,6 +45,8 @@ At first we used a tuple that became longer and longer. We even had statistics b
 the wrong element of the tuple. Therefore, we changed to a structure and kept some free spots.
 \<close>
 
+subsection \<open>Search Information\<close>
+
 type_synonym search_stats = \<open>64 word \<times> 64 word \<times>64 word \<times> 64 word \<times> 64 word \<times> 64 word \<times>64 word \<times> 64 word \<times> 64 word \<times> 64 word \<times> 64 word \<times> 64 word\<close>
 
 definition Search_Stats_propagations :: \<open>search_stats \<Rightarrow> 64 word\<close> where
@@ -139,7 +141,10 @@ definition Search_Stats_set_ticks_focused :: \<open>64 word \<Rightarrow> search
 
 definition Search_Stats_incr_ticks_focused :: \<open>64 word \<Rightarrow> search_stats \<Rightarrow> search_stats\<close> where
   \<open>Search_Stats_incr_ticks_focused = (\<lambda>t (propa, confl, dec, res, reduction, uset, gcs, units, irred_cls, no_conflict_until, ticks, ticks_focused). (propa, confl, dec, res, reduction, uset, gcs, units, irred_cls, no_conflict_until, ticks, ticks_focused+t))\<close>
-  
+
+
+subsection \<open>Inprocessing Information\<close>
+
 type_synonym inprocessing_binary_stats = \<open>64 word \<times> 64 word \<times> 64 word\<close>
 
 definition Binary_Stats_incr_rounds :: \<open>inprocessing_binary_stats \<Rightarrow> inprocessing_binary_stats\<close> where
@@ -200,6 +205,9 @@ definition Pure_lits_Stats_incr_rounds :: \<open>inprocessing_pure_lits_stats \<
 definition Pure_lits_Stats_incr_removed :: \<open>inprocessing_pure_lits_stats \<Rightarrow> inprocessing_pure_lits_stats\<close> where
   \<open>Pure_lits_Stats_incr_removed = (\<lambda>(rounds, removed). (rounds, removed+1))\<close>
 
+
+subsubsection \<open>Biggest Seen Clause\<close>
+
 type_synonym lbd_size_limit_stats = \<open>nat \<times> nat\<close>
 
 definition LSize_Stats_lbd where
@@ -211,7 +219,9 @@ definition LSize_Stats_size where
 definition LSize_Stats where
   \<open>LSize_Stats lbd size' = (lbd, size')\<close>
 
-
+  
+subsubsection \<open>Rephasing\<close>
+  
 type_synonym rephase_stats = \<open>64 word \<times> 64 word \<times> 64 word \<times> 64 word \<times> 64 word \<times> 64 word\<close>
 
 definition Rephase_Stats_total :: \<open>rephase_stats \<Rightarrow> _\<close> where
@@ -220,15 +230,40 @@ definition Rephase_Stats_total :: \<open>rephase_stats \<Rightarrow> _\<close> w
 definition Rephase_Stats_incr_total :: \<open>rephase_stats \<Rightarrow> rephase_stats\<close> where
   \<open>Rephase_Stats_incr_total = (\<lambda>(rephased, original, best, invert, flipped, random). (rephased+1, original, best, invert, flipped, random))\<close>
 
+
+subsubsection \<open>Rate\<close>
+
+text \<open>Rate = number of decision between conflicts. If the number is too high, then we should not do
+ recursive bumping, especially since our sorting is less efficient than the one in kissat.\<close>
+
+type_synonym isasat_rate = \<open>(ema \<times> ema \<times> 64 word)\<close>
+
+definition Rate_get_rate :: \<open>bool \<Rightarrow> isasat_rate \<Rightarrow> 64 word\<close> where
+  \<open>Rate_get_rate is_stable = (\<lambda>(rate_focused, rate_stable, last_decision). if is_stable then ema_extract_value rate_stable else ema_extract_value rate_focused)\<close>
+
+definition Rate_get_rate_last_decision :: \<open>isasat_rate \<Rightarrow> 64 word\<close> where
+  \<open>Rate_get_rate_last_decision = (\<lambda>(rate_focused, rate_stable, last_decision). last_decision)\<close>
+
+definition Rate_set_rate_last_decision :: \<open>64 word \<Rightarrow> isasat_rate \<Rightarrow> isasat_rate\<close> where
+  \<open>Rate_set_rate_last_decision last_decision  = (\<lambda>(rate_focused, rate_stable, _). (rate_focused, rate_stable, last_decision))\<close>
+
+definition Rate_update_rate :: \<open>bool \<Rightarrow> 64 word \<Rightarrow> isasat_rate \<Rightarrow> isasat_rate\<close> where
+  \<open>Rate_update_rate is_stable r = (\<lambda>(rate_focused, rate_stable, last_decision).
+  (if is_stable then rate_focused else ema_update_word (r - last_decision) rate_focused,
+   if is_stable then ema_update_word  (r - last_decision) rate_stable else rate_stable, r))\<close>
+
+
+subsection \<open>All Together\<close>
+
 type_synonym isasat_stats = \<open>
   (search_stats, inprocessing_binary_stats, inprocessing_subsumption_stats, ema,
   inprocessing_pure_lits_stats, lbd_size_limit_stats,
   rephase_stats,
+  isasat_rate,
 
-  64 word,
   64 word, 64 word,64 word, 64 word,
   64 word, 64 word, 32 word, 64 word) tuple16\<close>
-text \<open>The unused part starts after the linebreak, but Isabelle does not allow for comments there.\<close>
+text \<open>The unused part starts after the line break, but Isabelle does not allow for comments there.\<close>
 
 
 abbreviation Stats :: \<open>_ \<Rightarrow> _ \<Rightarrow>_ \<Rightarrow> _ \<Rightarrow>_ \<Rightarrow> _ \<Rightarrow>_ \<Rightarrow> _ \<Rightarrow>_ \<Rightarrow> _ \<Rightarrow>_ \<Rightarrow> _ \<Rightarrow>_ \<Rightarrow> _ \<Rightarrow>_ \<Rightarrow> _ \<Rightarrow> isasat_stats\<close> where
@@ -255,6 +290,9 @@ definition get_lsize_limit_stats :: \<open>isasat_stats \<Rightarrow> lbd_size_l
 definition get_rephase_stats :: \<open>isasat_stats \<Rightarrow> rephase_stats\<close> where
   \<open>get_rephase_stats \<equiv> Tuple16.Tuple16_get_g\<close>
 
+definition get_rate_stats :: \<open>isasat_stats \<Rightarrow> isasat_rate\<close> where
+  \<open>get_rate_stats \<equiv> Tuple16.Tuple16_get_h\<close>
+
 definition set_propagation_stats :: \<open>search_stats \<Rightarrow> isasat_stats \<Rightarrow> isasat_stats\<close> where
   \<open>set_propagation_stats \<equiv> Tuple16.set_a\<close>
 
@@ -276,6 +314,9 @@ definition set_lsize_limit_stats :: \<open>lbd_size_limit_stats \<Rightarrow> is
 definition set_rephase_stats :: \<open>rephase_stats \<Rightarrow> isasat_stats \<Rightarrow> isasat_stats\<close> where
   \<open>set_rephase_stats \<equiv> Tuple16.set_g\<close>
 
+definition set_rate_stats :: \<open>isasat_rate \<Rightarrow> isasat_stats \<Rightarrow> isasat_stats\<close> where
+  \<open>set_rate_stats \<equiv> Tuple16.set_h\<close>
+  
 definition incr_propagation :: \<open>isasat_stats \<Rightarrow> isasat_stats\<close> where
   \<open>incr_propagation S = (set_propagation_stats (Search_Stats_incr_propagation (get_search_stats S)) S)\<close>
 
@@ -294,6 +335,9 @@ definition incr_conflict :: \<open>isasat_stats \<Rightarrow> isasat_stats\<clos
 definition incr_decision :: \<open>isasat_stats \<Rightarrow> isasat_stats\<close> where
   \<open>incr_decision S = (set_propagation_stats (Search_Stats_incr_decisions (get_search_stats S)) S)\<close>
 
+definition get_decisions :: \<open>isasat_stats \<Rightarrow> 64 word\<close> where
+  \<open>get_decisions S = (Search_Stats_decisions (get_search_stats S))\<close>
+  
 definition incr_restart :: \<open>isasat_stats \<Rightarrow> isasat_stats\<close> where
   \<open>incr_restart S = (set_propagation_stats (Search_Stats_incr_restarts (get_search_stats S)) S)\<close>
 
@@ -474,6 +518,22 @@ definition stats_size_limit :: \<open>isasat_stats \<Rightarrow> nat\<close> whe
 definition set_stats_size_limit :: \<open>nat \<Rightarrow> nat \<Rightarrow> isasat_stats \<Rightarrow> isasat_stats\<close> where
   \<open>set_stats_size_limit lbd size' = set_lsize_limit_stats (lbd, size')\<close>
 
+context begin
+qualified definition BUMPREASONRATE where
+  \<open>BUMPREASONRATE = 10\<close> (*Kissat has 10, but our sorting is worse, so maybe decrease*)
+
+qualified definition rate_should_bump_reason :: \<open>bool \<Rightarrow> isasat_stats \<Rightarrow> bool\<close> where
+  \<open>rate_should_bump_reason is_stable stats = (Rate_get_rate is_stable (get_rate_stats stats) \<ge> BUMPREASONRATE)\<close>
+
+qualified definition update_rate :: \<open>bool \<Rightarrow> 64 word \<Rightarrow> isasat_stats \<Rightarrow> isasat_stats\<close> where
+  \<open>update_rate is_stable dec stats = (set_rate_stats (Rate_update_rate is_stable dec (get_rate_stats stats)) stats)\<close>
+
+qualified definition rate_set_last_decision :: \<open>64 word \<Rightarrow> isasat_stats \<Rightarrow> isasat_stats\<close> where
+  \<open>rate_set_last_decision dec stats = (set_rate_stats (Rate_set_rate_last_decision dec (get_rate_stats stats)) stats)\<close>
+
+
+end
+
 
 section \<open>Information related to restarts\<close>
 
@@ -512,12 +572,14 @@ definition restart_info_restart_done :: \<open>restart_info \<Rightarrow> restar
 definition empty_stats :: \<open>isasat_stats\<close> where
   \<open>empty_stats = Tuple16( (0,0,0,0,0,0,0,0,0,0,0,0)::search_stats)
   ((0,0,0)::inprocessing_binary_stats) ((0,0,0,0,0)::inprocessing_subsumption_stats)
-  (ema_fast_init::ema) ((0,0)::inprocessing_pure_lits_stats) (0,0) (0,0,0,0,0,0) 0 0 0 0 0 0 0 0 0\<close>
+  (ema_fast_init::ema) ((0,0)::inprocessing_pure_lits_stats) (0,0) (0,0,0,0,0,0)
+  ((ema_fast_init, ema_fast_init, 0)::isasat_rate) 0 0 0 0 0 0 0 0\<close>
 
 definition empty_stats_clss :: \<open>64 word \<Rightarrow> isasat_stats\<close> where
   \<open>empty_stats_clss n = Tuple16( (0,0,0,0,0,0,0,0,n,0,0,0)::search_stats)
   ((0,0,0)::inprocessing_binary_stats) ((0,0,0,0,0)::inprocessing_subsumption_stats)
-  (ema_fast_init::ema) ((0,0)::inprocessing_pure_lits_stats) (0,0) (0,0,0,0,0,0) 0 0 0 0 0 0 0 0 0\<close>
+  (ema_fast_init::ema) ((0,0)::inprocessing_pure_lits_stats) (0,0) (0,0,0,0,0,0)
+  ((ema_fast_init, ema_fast_init, 0)::isasat_rate) 0 0 0 0 0 0 0 0\<close>
 
 
 section \<open>Scheduling Information\<close>
