Weidenbach_Book/IsaSAT/IsaSAT_EMA.thy
@@ -39,6 +39,22 @@ definition (in -) ema_update :: \<open>nat \<Rightarrow> ema \<Rightarrow> ema\<
        let \<beta> = if \<beta> < \<alpha> then \<alpha> else \<beta> in
        (value, \<alpha>, \<beta>, wait, period))\<close>
 
+definition (in -) ema_update_word :: \<open>64 word \<Rightarrow> ema \<Rightarrow> ema\<close> where
+  \<open>ema_update_word = (\<lambda>lbd (value, \<alpha>, \<beta>, wait, period).
+     let lbd = (lbd) * ema_bitshifting in
+     let value = if lbd > value
+        then value + ((\<beta> >> (EMA_FIXPOINT_SIZE - EMA_MULT_SHIFT)) * ((lbd - value) >> EMA_MULT_SHIFT))
+        else value - ((\<beta> >> (EMA_FIXPOINT_SIZE - EMA_MULT_SHIFT)) * ((value - lbd) >> EMA_MULT_SHIFT))
+     in
+     let wait = wait - 1 in
+       if \<beta> \<le> \<alpha> \<or> wait > 0 then (value, \<alpha>, \<beta>, wait, period)
+     else
+       let wait = 2 * (period+1)-1 in
+       let period = wait in
+       let \<beta> = \<beta> >> 1 in
+       let \<beta> = if \<beta> < \<alpha> then \<alpha> else \<beta> in
+       (value, \<alpha>, \<beta>, wait, period))\<close>
+
 definition (in -) ema_init :: \<open>64 word \<Rightarrow> ema\<close> where
   \<open>ema_init \<alpha> = (0, \<alpha>  >> (EMA_FIXPOINT_SIZE - 32), ema_bitshifting, 1, 0)\<close>
 
